proof/DDC/Language/SimpleData/StepAlt.v
@@ -1,15 +1,15 @@
 
-Require Export TyJudge.
-Require Export Exp.
-Require Export SubstExpExp.
+Require Export DDC.Language.SimpleData.TyJudge.
+Require Export DDC.Language.SimpleData.Exp.
+Require Export DDC.Language.SimpleData.SubstExpExp.
 
 
 
-Lemma getAltExp_good
+Lemma getAlt_good
  :  forall ds te tPat tResult alts dc tsArgs x
  ,  Forall (fun a => TYPEA ds te a tPat tResult) alts
  -> In (AAlt dc tsArgs x) alts
- -> TYPE ds (te ++ envOfList tsArgs) x tResult.
+ -> TYPE ds (te >< tsArgs) x tResult.
 Proof.
  intros.
  rewrite Forall_forall in H.
@@ -17,17 +17,17 @@ Proof.
 Qed.
 
 
-Lemma getAltExp_inAlts
+Lemma getAlt_inAlts
  :  forall ds te tResult tCon alts dc tsArgs x1 x2
  ,  TYPE ds te (XCase x1 alts) tResult
  -> getDataDef dc ds   = Some (DefData dc tsArgs tCon)
  -> getAlt     dc alts = Some (AAlt    dc tsArgs x2)
- -> TYPE ds (te ++ envOfList tsArgs) x2 tResult.
+ -> TYPE ds (te >< tsArgs) x2 tResult.
 Proof.
  intros.
  inverts keep H.
- lets HA:  getAltExp_hasAlt H1.
- lets HXT: getAltExp_good H5 HA.
+ lets HA:  getAlt_in H1.
+ lets HXT: getAlt_good H5 HA.
  auto.
 Qed.
  
@@ -41,7 +41,7 @@ Lemma getAlt_matches_dataDef
 Proof.
  intros.
  rewrite Forall_forall in H.
- lets D: getAltExp_hasAlt H1.
+ lets D: getAlt_in H1.
  apply H in D.
  inverts D.
  rewrite H0 in H9.
