proof/DDC/Language/SimpleData/SubstExpExp.v
@@ -1,27 +1,28 @@
 
-Require Import TyJudge.
-Require Export Exp.
+Require Import DDC.Language.SimpleData.TyJudge.
+Require Import DDC.Language.SimpleData.ExpSubst.
+Require Export DDC.Language.SimpleData.Exp.
+
 
 (* Substitution of values in values. 
    Inductively, we must reason about performing substitutions at any
    depth, hence we must prove a property about (subst' d x2 x1) instead
    of the weaker (subst x2 x1) which assumes the substitution is taking
-   place at top level.
- *)
-Theorem subst_value_value_ix
+   place at top level. *)
+Theorem subst_exp_exp_ix
  :  forall ix ds te x1 x2 t1 t2
- ,  get  te ix = Some t2
+ ,  get  ix te = Some t2
  -> TYPE ds te           x1 t1
- -> TYPE ds (drop ix te) x2 t2
- -> TYPE ds (drop ix te) (substX ix x2 x1) t1.
+ -> TYPE ds (delete ix te) x2 t2
+ -> TYPE ds (delete ix te) (substX ix x2 x1) t1.
 Proof.
  intros. gen ix ds te x2 t1 t2.
  induction x1 using exp_mutind with 
   (PA := fun a1 => forall ix ds te x2 t11 t12 t2
-      ,  get te ix = Some t2
+      ,  get ix te = Some t2
       -> TYPEA ds te           a1 t11 t12
-      -> TYPE  ds (drop ix te) x2 t2
-      -> TYPEA ds (drop ix te) (substA ix x2 a1) t11 t12)
+      -> TYPE  ds (delete ix te) x2 t2
+      -> TYPEA ds (delete ix te) (substA ix x2 a1) t11 t12)
   ; intros; simpl.
 
  Case "XVar".
@@ -33,19 +34,19 @@ Proof.
   SCase "n < ix".
    apply TYVar.
    rewrite <- H5.
-    apply get_drop_above. auto.
+    apply get_delete_above. auto.
 
   SCase "n > ix".
    apply TYVar.
    destruct n.
     false. omega.
     simpl. nnat. rewrite <- H5.
-     apply get_drop_below. omega.
+     apply get_delete_below. omega.
 
  Case "XLam".
   inverts H0.
   apply TYLam.
-  rewrite drop_rewind.
+  rewrite delete_rewind.
   eapply IHx1; eauto.
    simpl. apply type_tyenv_weaken1. auto.
 
@@ -56,8 +57,8 @@ Proof.
   inverts H0.
   eapply TYCon; eauto.
    rewrite Forall_forall in H.
-   apply (Forall2_map_left (TYPE ds (drop ix te))).
-   apply (Forall2_impl_In  (TYPE ds te)); eauto.
+   apply (Forall2_map_left (TYPE ds (delete ix te))).
+   apply (Forall2_impl_in  (TYPE ds te)); eauto.
 
  Case "XCase".
   inverts H0.
@@ -65,7 +66,7 @@ Proof.
    eauto. clear IHx1.
    rewrite Forall_forall in H.
    eapply Forall_map.
-   eapply (Forall_impl_In 
+   eapply (Forall_impl_in 
     (fun a => TYPEA ds te a (TCon tcPat) t1)); eauto.
    rewrite map_length. auto. eauto.
 
@@ -76,40 +77,40 @@ Proof.
     apply in_map_iff in H0.
      destruct H0. exists x. inverts H0.
      split; auto.
+     unfold compose.
      rewrite dcOfAlt_substA. auto.
      
  Case "AAlt".
   inverts H0.
   eapply TYAlt. 
    eauto.
-   rewrite drop_append.
-    rewrite <- length_envOfList.
+   rewrite delete_app.
     eapply IHx1 with (t2 := t2).
      auto.
-     rewrite <- (get_append_right_some ty ix te (envOfList ts)). 
+     rewrite <- (get_app_left_some ty ix te ts). 
       auto. auto.
-     rewrite <- drop_append.
+     rewrite <- delete_app.
       apply type_tyenv_weaken_append. eauto.
 Qed.
 
 
-Theorem subst_value_value
+Theorem subst_exp_exp
  :  forall ds te x1 x2 t1 t2
  ,  TYPE ds (te :> t2) x1 t1
  -> TYPE ds te         x2 t2 
  -> TYPE ds te (substX 0 x2 x1) t1.
 Proof. 
  intros ds te x1 x2 t1 t2 Ht1 Ht2.
- lets H: subst_value_value_ix 0 (te :> t2).
+ lets H: subst_exp_exp_ix 0 (te :> t2).
   simpl in H. eauto.
 Qed.
 
 
 (* Substitution of several expressions at once. *)
-Theorem subst_value_value_list
+Theorem subst_exp_exp_list
  :  forall ds te x1 xs t1 ts
  ,  Forall2 (TYPE ds te)         xs ts
- -> TYPE ds (te ++ envOfList ts) x1 t1
+ -> TYPE ds (te >< ts) x1 t1
  -> TYPE ds te    (substXs 0 xs x1) t1.
 Proof.
  intros ds te x1 xs t1 ts HF HT.
@@ -128,12 +129,12 @@ Proof.
     inverts HF.
     eapply IHxs. eauto.
     simpl in HT.
-    eapply subst_value_value. eauto.
-    assert (List.length xs = List.length ts).
-     eapply Forall2_length. eauto.
-    rewrite H. clear H.
-    rewrite <- length_envOfList.
-    eapply type_tyenv_weaken_append.
-    auto.
+    eapply subst_exp_exp. 
+     eauto.
+     assert (length xs = length ts).
+      eapply Forall2_length in H4. auto.   
+     rewrite H. clear H.
+     eapply type_tyenv_weaken_append.
+     auto.
 Qed.
 
